# limes

## Formulars

$$
f'(x_0)= \lim\limits_{h \to 0} \frac{f(x_0+h)-f(x_0)}{h}
$$

---

$$
f'(x_0)= \lim\limits_{h \to 0} \frac{f(x_0+h)-f(x_0)}{h}
$$

## examples

$$
f(x)=2x^2+3 \qquad\quad x_0 = 1
$$

NR:

$$
f(1)= 2 \times 1^2+3 = 5
$$

NR:

$$
f(1+h) = 2 \times (1+h)^2+3\\
f(1+h) = 2 \times (1+2h+h^2)+3\\
f(1+h) = 2+4h+2h^2+3\\
f(1+h) = 5+4h+2h^2
$$

<br>

$$
f'(x_0)= \lim\limits_{h \to 0} \frac{f(x_0+h)-f(x_0)}{h}\\
f'(x_0)= \lim\limits_{h \to 0} \frac{5+4h+2h^2-5}{h}\\
= \lim\limits_{h \to 0} \frac{4h+2h^2}{h}\\
= \lim\limits_{h \to 0} \frac{h\times(4+2h)}{h}\\
= \lim\limits_{h \to 0} 4+2h = 4
$$
